ML_SP_Graph.v
@@ -1,0 +1,413 @@
+(***************************************************************************
+* Preservation and Progress for mini-ML (CBV) - Graph handling             *
+* Jacques Garrigue, 2021                                                   *
+***************************************************************************)
+
+Set Implicit Arguments.
+Require Import Arith List Lia.
+Require Import Metatheory ML_SP_Definitions ML_SP_Infrastructure.
+
+Module MkGraph(Cstr:CstrIntf)(Const:CstIntf).
+
+Module Infra := MkInfra(Cstr)(Const).
+Import Infra Defs.
+
+(* Definitions *)
+
+Definition arrow_kind (m n : nat) :=
+  Kind Cstr.valid_arrow
+       (coherent_pair (T:=typ_bvar m) (T':=typ_bvar n) Cstr.arrow_attrs).
+Definition eq_kind (m n : nat) :=
+  Kind Cstr.valid_eq
+       (coherent_pair (T:=typ_bvar m) (T':=typ_bvar n) Cstr.eq_attrs).
+
+Fixpoint graph_of_tree ofs (tr : tree) : nat * list kind :=
+  match tr with
+  (* | tr_bvar n => (n, nil) *)
+  | tr_arrow t1 t2 =>
+    let '(n1, g1) := graph_of_tree (ofs + 1) t1 in
+    let '(n2, g2) := graph_of_tree (ofs + length g1 + 1) t2 in
+    (ofs, (Some (arrow_kind n1 n2), nil) :: g1 ++ g2)
+  | tr_eq t1 t2 =>
+    let '(n1, g1) := graph_of_tree (ofs + 1) t1 in
+    let '(n2, g2) := graph_of_tree (ofs + length g1 + 1) t2 in
+    (ofs, (Some (eq_kind n1 n2), nil) :: g1 ++ g2)
+  | tr_rvar rv =>
+    (ofs, (None, rv :: nil) :: nil)
+  | tr_stuck t1 _ =>
+    graph_of_tree ofs t1
+  end.
+
+Definition graph_of_tree_type S := graph_of_tree 0 S.
+
+Definition annotation_tree (S : tree) := tr_arrow S S.
+
+(*
+Fixpoint graph_of_kinds ofs (Ks : list tree_kind) : list kind * list kind :=
+  match Ks with
+  | nil => (nil, nil)
+  | (None,rvs) :: rem =>
+    let '(K, K') := graph_of_kinds ofs rem in
+    ((None,rvs) :: K, K')
+  | (Some(kc,kr),rvs) :: rem =>
+    let K' := fold_left
+                (fun K' atr =>
+                   let '(_, K'') :=
+                       graph_of_tree (ofs + length K') (snd atr) in
+                   K' ++ K'')
+                kr nil
+    in
+    let '(K, K'') := graph_of_kinds (ofs + length K') rem in
+    (K, K' ++ K'')
+  end.
+  
+Definition graph_of_tree_type (S : tree_type) : nat * list kind :=
+  let '(T,Ks) := S in
+  let '(K,K') := graph_of_kinds (length Ks) Ks in
+  let '(n,K'') := graph_of_tree (length K + length K') T in
+  (n, K ++ K' ++ K'').
+
+Eval compute in
+  graph_of_tree_type (tr_arrow (tr_rvar (rvar_b 0)) (tr_rvar (rvar_b 1)), nil).
+
+Definition static_tree_kind (k : tree_kind) :=
+  match k with
+  | (None,nil) => false
+  | (None,_) => true
+  | (Some (kc,kr),_) => Cstr.static kc
+  end.
+
+Fixpoint build_right_map pos ofs (Ks : list tree_kind) n :=
+  match Ks with
+  | nil => n
+  | k :: rem =>
+    if static_tree_kind k then
+      if n === pos then ofs else build_right_map (S pos) (S ofs) rem n
+    else build_right_map (S pos) ofs rem n
+  end.
+
+Section right_tree.
+Variable V : nat -> nat.
+Fixpoint bsubst_tree (T : tree) :=
+  match T with
+  (* | tr_bvar x => tr_bvar (V x) *)
+  | tr_arrow T U => tr_arrow (bsubst_tree T) (bsubst_tree U)
+  | tr_eq T U => tr_eq (bsubst_tree T) (bsubst_tree U)
+  | tr_rvar r => T
+  end.
+
+Definition bsubst_tree_kind (k : tree_kind) :=
+  match k with
+  | (Some (c, trees), rvars) =>
+    (Some (c, List.map (fun p => (fst p, bsubst_tree (snd p))) trees), rvars)
+  | (None, rvars) => k
+  end.
+
+Definition right_tree_kinds :=
+  map (fun k => if static_tree_kind k then bsubst_tree_kind k else k).
+End right_tree.
+
+Definition annotation_tree (S : tree_type) :=
+  let '(T,K) := S in
+  let V := build_right_map 0 (length K) K in
+  (tr_arrow T (bsubst_tree T), K ++ right_tree_kinds K).
+*)
+
+(*
+Inductive lookup_rvar : rvar -> tree -> Prop :=
+  | lr_f : forall r T,
+      binds r T S ->
+      lookup_rvar (rvar_f r) T
+  | lr_attr_dom : forall rv T1 T2,
+      lookup_rvar rv (tr_arrow T1 T2) ->
+      lookup_rvar (rvar_attr rv Cstr.arrow_dom) T1
+  | lr_attr_cod : forall rv T1 T2,
+      lookup_rvar rv (tr_arrow T1 T2) ->
+      lookup_rvar (rvar_attr rv Cstr.arrow_cod) T2
+  | lr_attr_fst : forall rv T1 T2,
+      lookup_rvar rv (tr_eq T1 T2) ->
+      lookup_rvar (rvar_attr rv Cstr.eq_fst) T1
+  | lr_attr_snd : forall rv T1 T2,
+      lookup_rvar rv (tr_eq T1 T2) ->
+      lookup_rvar (rvar_attr rv Cstr.eq_snd) T2.
+
+Inductive tree_subst_eq : tree -> tree -> Prop :=
+  | tse_var1 : forall rv T1 T2,
+      lookup_rvar rv T1 ->
+      tree_subst_eq T1 T2 ->
+      tree_subst_eq (tr_rvar rv) T2
+  | tse_var2 : forall rv T1 T2,
+      lookup_rvar rv T2 ->
+      tree_subst_eq T1 T2 ->
+      tree_subst_eq T1 (tr_rvar rv)
+  | tse_arrow : forall T1 T2 T1' T2',
+      tree_subst_eq T1 T1' -> tree_subst_eq T2 T2' ->
+      tree_subst_eq (tr_arrow T1 T2) (tr_arrow T1' T2')
+  | tse_eq : forall T1 T2 T1' T2',
+      tree_subst_eq T1 T1' -> tree_subst_eq T2 T2' ->
+      tree_subst_eq (tr_eq T1 T2) (tr_eq T1' T2')
+  | tse_rvar : forall rv, tree_subst_eq (tr_rvar rv) (tr_rvar rv).
+*)
+
+Eval compute in
+  graph_of_tree_type (
+  annotation_tree (tr_arrow (tr_rvar (rvar_b 0)) (tr_rvar (rvar_b 1)))).
+
+(* Eval compute in
+  annotation_tree (tr_arrow (tr_rvar (rvar_b 0)) (tr_bvar 0),
+                   (None, rvar_b 1 :: nil) :: nil). 
+
+Eval compute in
+  graph_of_tree_type (
+  annotation_tree (tr_arrow (tr_rvar (rvar_b 0)) (tr_bvar 0),
+                   (None, rvar_b 1 :: nil) :: nil)). *)
+
+(*
+\/ 'a::int, 'b. eq('a, 'b)
+Sch (tr_eq (tr_bvar 0) (tr_bvar 1)) [({sch_cstr:=int;...},nil); (None,nil)]
+
+[({sch_cstr:=int;...},nil); (None,nil); ({sch_cstr:=int;...},nil)]
+Vl : 0 => 0, 1 => 1
+Vr : 0 => 2, 1 => 1
+
+graph_of_tree Vl 3 s = (3, [(eq,{fst=>typ_bvar 0; snd=>typ_bar 2},nil)]) 
+graph_of_tree Vr 4 s = (4, [(eq,{fst=>typ_bvar 1; snd=>typ_bar 2},nil)])
+(typ_bvar 5,
+[({sch_cstr:=int;...},nil); (None,nil); ({sch_cstr:=int;...},nil);
+ (eq,{fst=>typ_bvar 0; snd=>typ_bvar 1},nil);
+ (eq,{fst=>typ_bvar 2; snd=>typ_bvar 1},nil);
+ (arrow,{left=>typ_bvar 3; right=> typ_bvar 4}, nil)]
+*)
+
+(** Check if there are free rigid variables *)
+Fixpoint rclosed_rvar (r : rvar) : Prop :=
+  match r with
+  | rvar_b _ => False
+  | rvar_f _ => True
+  | rvar_attr l a => rclosed_rvar l
+  end.
+
+Fixpoint rclosed_tree (T : tree) : Prop :=
+  match T with
+  | tr_arrow T1 T2 | tr_eq T1 T2 => rclosed_tree T1 /\ rclosed_tree T2
+  | tr_rvar r => rclosed_rvar r
+  | tr_stuck T1 a => rclosed_tree T1
+  end.
+
+Fixpoint rclosed (t : trm) : Prop :=
+  match t with
+  | trm_eq | trm_bvar _ | trm_fvar _ | trm_cst _ => True
+  | trm_abs t' => rclosed t'
+  | trm_let t1 t2 | trm_app t1 t2 => rclosed t1 /\ rclosed t2
+  | trm_use t1 T1 T2 t2 =>
+    rclosed t1 /\ rclosed t2 /\
+    rclosed_tree T1 /\ rclosed_tree T2
+  | trm_rigid t => rclosed t
+  | trm_ann t T => rclosed t /\ rclosed_tree T
+  end.
+
+(* Infrastructure *)
+
+Lemma graph_of_tree_n m T :
+  let '(n, Ks) := graph_of_tree m T in
+  n < length Ks + m.
+Proof.
+  revert m. induction T; intros; simpl*.
+  case_eq (graph_of_tree (m + 1) T1); intros.
+  case_eq (graph_of_tree (m + length l + 1) T2); intros.
+  simpl*. lia.
+  case_eq (graph_of_tree (m + 1) T1); intros.
+  case_eq (graph_of_tree (m + length l + 1) T2); intros.
+  simpl*. lia.
+  apply IHT.
+Qed.
+  
+Lemma graph_of_tree_type_n T :
+  let '(n, Ks) := graph_of_tree_type T in
+  n < length Ks.
+Proof.
+  unfold graph_of_tree_type.
+  case_eq (graph_of_tree 0 T); intros.
+  generalize (graph_of_tree_n 0 T).
+  rewrite H. lia.
+Qed.
+
+(* Soundness *)
+
+Lemma graph_of_tree_subst ofs tr S :
+  let Ks := snd (graph_of_tree ofs tr) in
+  List.map (kind_subst S) Ks = Ks.
+Proof.
+  revert ofs; induction tr; simpl; intros; auto.
+  - specialize (IHtr1 (ofs+1)); revert IHtr1.
+    case_eq (graph_of_tree (ofs + 1) tr1); simpl; introv Htr1 IHtr1.
+    specialize (IHtr2 (ofs+length l+1)); revert IHtr2.
+    case_eq (graph_of_tree (ofs + length l + 1) tr2); simpl; introv Htr2 IHtr2.
+    rewrite map_app, IHtr1, IHtr2.
+    unfold kind_subst, kind_map.
+    f_equal.
+    f_equal.
+    now apply kind_pi.
+  - specialize (IHtr1 (ofs+1)); revert IHtr1.
+    case_eq (graph_of_tree (ofs + 1) tr1); simpl; introv Htr1 IHtr1.
+    specialize (IHtr2 (ofs+length l+1)); revert IHtr2.
+    case_eq (graph_of_tree (ofs + length l + 1) tr2); simpl; introv Htr2 IHtr2.
+    rewrite map_app, IHtr1, IHtr2.
+    unfold kind_subst, kind_map.
+    f_equal.
+    f_equal.
+    now apply kind_pi.
+Qed.
+
+Lemma graph_of_tree_type_subst n Ks tr S :
+  graph_of_tree_type tr = (n, Ks) ->
+  List.map (kind_subst S) Ks = Ks.
+Proof.
+  unfold graph_of_tree_type.
+  case_eq (graph_of_tree 0 tr); introv HK E.
+  injection E; intros; subst.
+  generalize (graph_of_tree_subst 0 tr S); simpl.
+  now rewrite HK.
+Qed.
+
+(*
+Lemma graph_of_kinds_subst ofs TKs S :
+  let (Ks, Ks') := graph_of_kinds ofs TKs in
+  List.map (kind_subst S) Ks = Ks /\ List.map (kind_subst S) Ks' = Ks'.
+Proof.
+  revert ofs.
+  induction TKs; simpl; intros; auto.
+  destruct a as [[[]|] rvs].
+    set (ofs' := ofs + _).
+    specialize (IHTKs ofs'); revert IHTKs.
+    case_eq (graph_of_kinds ofs' TKs); introv HG; intros [E1 E2].
+    splits*.
+    rewrite map_app, E2.
+    f_equal.
+    assert (List.map (kind_subst S) nil = nil) by auto.
+    revert H; generalize (@nil kind).
+    clear; induction l; simpl; intros; auto.
+    generalize (graph_of_tree_subst (ofs + length l0) (snd a) S).
+    case_eq (graph_of_tree (ofs + length l0) (snd a)); simpl; intros.
+    apply IHl.
+    now rewrite map_app, H, H1.
+  specialize (IHTKs ofs); revert IHTKs.
+  case_eq (graph_of_kinds ofs TKs); simpl; introv HG; intros [E1 E2].
+  unfold kind_subst at 1, kind_map; simpl.
+  now rewrite E1, E2.
+Qed.
+
+Lemma graph_of_tree_type_subst n Ks tr S :
+  graph_of_tree_type tr = (n, Ks) ->
+  List.map (kind_subst S) Ks = Ks.
+Proof.
+  simpl.
+  unfold graph_of_tree_type.
+  destruct tr as [T K].
+  generalize (graph_of_kinds_subst (length K) K S).
+  case_eq (graph_of_kinds (length K) K); simpl; introv HG; intros [E1 E2].
+  generalize (graph_of_tree_subst (length l + length l0) T S).
+  case_eq (graph_of_tree (length l + length l0) T); simpl; introv HT E E'.
+  injection E'; intros; subst.
+  now rewrite map_app, map_app, E1, E2, E.
+Qed.
+*)
+
+Section set_nth.
+Variable A : Type.
+Fixpoint set_nth (n : nat) (x : A) l def :=
+  match n with
+  | 0 => x :: tl l
+  | S n => hd def l :: set_nth n x (tl l) def
+  end.
+
+Lemma set_nth_same n x l def def' : nth n (set_nth n x l def) def' = x.
+Proof. revert l; induction n; simpl*. Qed.
+
+Lemma set_nth_other n' x l def n :
+  n' <> n -> nth n (set_nth n' x l def) def = nth n l def.
+Proof.
+revert n l; induction n'; destruct l; destruct n; simpl; intros; auto;
+  try contradiction.
+- now destruct n.
+- rewrite IHn'. now destruct n. intro N; elim H; now rewrite N.
+Qed.
+
+Lemma length_set_nth n x l def : length l <= length (set_nth n x l def).
+Proof.
+  revert n; induction l; simpl; intros; auto with arith.
+  destruct n; simpl; auto with arith.
+Qed.
+End set_nth.
+
+Lemma extract_unique_attr K V k rvs k' rvs' a T S n Ks Us :
+  binds V (Some k, rvs) K ->
+  proper_instance K Ks Us ->
+  nth n Us typ_def = typ_fvar V ->
+  nth n Ks (None, nil) = (Some k', rvs') ->
+  In (a, T) (kind_rel k) ->
+  In (a, S) (kind_rel k') ->
+  Cstr.unique (kind_cstr k) a = true ->
+  typ_open S Us = T.
+Proof.
+  intros B PI nUs nKs HT HS HU.
+  apply (@kind_coherent k a); auto.
+  destruct PI.
+  destruct (le_lt_dec (length Ks) n).
+    rewrite (nth_overflow _ _ l) in nKs; discriminate.
+  forward~ (list_forall2_nth (n:=n) (kind_open (Some k', rvs') nil) typ_def H0)
+      as WK.
+    unfold kinds_open; now rewrite map_length.
+  inversions WK; clear WK.
+  rewrite nUs in H1; inversions H1; clear H1.
+  puts (binds_func B H2); subst.
+  destruct H3. revert H1.
+  unfold kinds_open; simpl.
+  rewrite (nth_indep _ _ (kind_open (None, nil) Us));
+    try now rewrite map_length.
+  rewrite (map_nth (fun k => kind_open k Us)), nKs.
+  simpl; intros [_ Erel].
+  forward~ (Erel (a, typ_open S Us)).
+  rewrite kind_rel_map.
+  now apply (in_map_snd (fun T => typ_open T Us)).
+Qed.
+
+Lemma graph_of_tr_arrow n Ks ofs T1 T2 :
+  graph_of_tree ofs (tr_arrow T1 T2) = (n, Ks) ->
+  exists m1, exists Ks1, exists m2, exists Ks2,
+      Ks = (Some (arrow_kind m1 m2), nil) :: Ks1 ++ Ks2 /\
+      graph_of_tree (ofs+1) T1 = (m1, Ks1) /\
+      graph_of_tree (ofs+length Ks1+1) T2 = (m2, Ks2).
+Proof.
+  simpl.
+  case_eq (graph_of_tree (ofs + 1) T1); intros m1 Ks1 HT1.
+  case_eq (graph_of_tree (ofs + length Ks1 + 1) T2); intros m2 Ks2 HT2 E.
+  inversions E; clear E.
+  now repeat esplit.
+Qed.
+
+Lemma graph_of_tr_eq n Ks ofs T1 T2 :
+  graph_of_tree ofs (tr_eq T1 T2) = (n, Ks) ->
+  exists m1, exists Ks1, exists m2, exists Ks2,
+      Ks = (Some (eq_kind m1 m2), nil) :: Ks1 ++ Ks2 /\
+      graph_of_tree (ofs+1) T1 = (m1, Ks1) /\
+      graph_of_tree (ofs+length Ks1+1) T2 = (m2, Ks2).
+Proof.
+  simpl.
+  case_eq (graph_of_tree (ofs + 1) T1); intros m1 Ks1 HT1.
+  case_eq (graph_of_tree (ofs + length Ks1 + 1) T2); intros m2 Ks2 HT2 E.
+  inversions E; clear E.
+  now repeat esplit.
+Qed.
+
+Lemma graph_of_tree_root n Ks ofs T :
+  graph_of_tree ofs T = (n, Ks) -> n = ofs.
+Proof.
+  induction T; simpl; try solve [introv E; inversions* E];
+  try solve[ simpl;
+             case_eq (graph_of_tree (ofs + 1) T1); intros n1 K1;
+             case_eq (graph_of_tree (ofs + length K1 + 1) T2); intros;
+             inversions* H1 ].
+Qed.
+
+End MkGraph.
